{
  "@context": {
    "schema": "http://schema.org/",
    "rdf": "http://www.w3.org/1999/02/22-rdf-syntax-ns#",
    "rdfs": "http://www.w3.org/2000/01/rdf-schema#",
    "bs": "https:/bioschemas.org/terms/",
    "codemeta": "https://w3id.org/codemeta/terms/",
    "m4ml": "https://discovery.biothings.io/view/m4ml/"
  },
  "@graph": [
    {
      "@id": "m4ml:MLSoftwareSourceCode",
      "@type": "rdfs:Class",
      "rdfs:comment": "A software source code used to create a machine learning model.",
      "rdfs:label": "MLSoftwareSourceCode",
      "rdfs:subClassOf": {
        "@id": "schema:SoftwareSourceCode"
      },
      "schemaVersion": [
        "https://schema.org/docs/releases.html#v23.0"
      ]
    },
    {
      "@id": "m4ml:MLSoftwareApplication",
      "@type": "rdfs:Class",
      "rdfs:comment": "A software application used to create a machine learning model.",
      "rdfs:label": "MLSoftwareApplication",
      "rdfs:subClassOf": {
        "@id": "schema:SoftwareApplication"
      },
      "schemaVersion": [
        "https://schema.org/docs/releases.html#v23.0"
      ]
    },
    {
      "@id": "m4ml:MLModel",
      "@type": "rdfs:Class",
      "rdfs:comment": "An 'executable' ML model that could be used by third-parties for direct use, deployment, fine-tuning, transfer learning, etc.",
      "rdfs:label": "MLModel",
      "rdfs:subClassOf": {
        "@id": "schema:SoftwareApplication"
      },
      "schemaVersion": [
        "https://schema.org/docs/releases.html#v23.0"
      ]
    },
    {
      "@id": "m4ml:MLModelOptimizationAction",
      "@type": "rdfs:Class",
      "rdfs:comment": "An particular execution of an MLSoftware (either SourceCode or Application) to generate an MLModel.",
      "rdfs:label": "MLModelOptimizationAction",
      "rdfs:subClassOf": {
        "@id": "schema:Action"
      },
      "schemaVersion": [
        "https://schema.org/docs/releases.html#v23.0"
      ]
    },
    {
      "@id": "m4ml:MLModelValidationAction",
      "@type": "rdfs:Class",
      "rdfs:comment": "An external validation done for an ML model.",
      "rdfs:label": "MLModelValidationAction",
      "rdfs:subClassOf": {
        "@id": "schema:Action"
      },
      "schemaVersion": [
        "https://schema.org/docs/releases.html#v23.0"
      ]
    },


    
    {
      "@id": "m4ml:deployedAt",
      "@type": "rdf:Property",
      "rdfs:comment": "Platform, website, webservice or similar where this ML model has been deployed. There could be deployments that this ML model is not aware of (e.g., done by third-parties).",
      "rdfs:label": "deployedAt",
      "schema:domainIncludes": [
        {
          "@id": "m4ml:MLModel"
        }
      ],
      "schema:rangeIncludes": [
         {
           "@id": "schema:Thing"
         }
      ]
    },
    {
      "@id": "m4ml:evaluationMetric",
      "@type": "rdf:Property",
      "rdfs:comment": "Evaluation metrics used by the software for the training process. As the same software can be used for multiple runs (e.g., to find the  best performing model), no actual values for the evaluation metrics should be specified here, only the metrics themselves. For instance precision (a positive number).",
      "rdfs:label": "evaluationMetric",
      "schema:domainIncludes": [
        {
          "@id": "m4ml:MLSoftwareSourceCode"
        },
        {
          "@id": "m4ml:MLSoftwareApplication"
        }
      ],
      "schema:rangeIncludes": [
        {
          "@id": "bs:FormalParameter"
        },
        {
          "@id": "schema:PropertyValue"
        }
      ]
    },
    {
      "@id": "m4ml:evaluationMetricValue",
      "@type": "rdf:Property",
      "rdfs:comment": "Evaluation metric values obtained when creating this ML model. There should be a correspondence with the evaluation metrics declared by the ML software used to create this ML model.",
      "rdfs:label": "evaluationMetricValue",
      "schema:domainIncludes": [
        {
          "@id": "m4ml:MLModel"
        },
        {
          "@id": "m4ml:MLModelValidationAction"
        }
      ],
      "schema:rangeIncludes": [
        {
          "@id": "schema:PropertyValue"
        }
      ]
    },
    {
      "@id": "m4ml:externalValidation",
      "@type": "rdf:Property",
      "rdfs:comment": "A validation action using this ML model with an external validation dataset (e.g., when new datasets are produced from experiments and were not used as part of the learning process of this ML model). There could be external validations that this ML model is not aware of (e.g., done by third-parties).",
      "rdfs:label": "externalValidation",
      "schema:domainIncludes": [
        {
          "@id": "m4ml:MLModel"
        }
      ],
      "schema:rangeIncludes": [
        {
          "@id": "m4ml:MLModelValidationAction"
        }
      ]
    },
    {
      "@id": "m4ml:fineTunedBy",
      "@type": "rdf:Property",
      "rdfs:comment": "ML Software fine-tuning this ML model.",
      "rdfs:label": "fineTunedBy",
      "schema:domainIncludes": [
        {
          "@id": "m4ml:MLModel"
        }
      ],
      "schema:rangeIncludes": [
         {
           "@id": "m4ml:MLSoftwareSourceCode"
         },
         {
          "@id": "m4ml:MLSoftwareApplication"
        }
      ]
    },
    {
      "@id": "m4ml:generatedBy",
      "@type": "rdf:Property",
      "rdfs:comment": "Optimization action on an ML software used to create this ML model.",
      "rdfs:label": "generatedBy",
      "schema:domainIncludes": [
        {
          "@id": "m4ml:MLModel"
        }
      ],
      "schema:rangeIncludes": [
         {
           "@id": "m4ml:MLOptimizationAction"
         }
      ]
    },
    {
      "@id": "m4ml:hyperparameter",
      "@type": "rdf:Property",
      "rdfs:comment": "Hyperparameters used by the software for the training process. As the same software can be used for multiple runs (e.g., to find the  best performing model), no actual values for the hyperparameters should be specified here, only the hyperparameters themselves. For instance windowSize (a number) or kernelSize (a number).",
      "rdfs:label": "hyperparameter",
      "schema:domainIncludes": [
        {
          "@id": "m4ml:MLSoftwareSourceCode"
        },
        {
          "@id": "m4ml:MLSoftwareApplication"
        }
      ],
      "schema:rangeIncludes": [
        {
          "@id": "bs:FormalParameter"
        },
        {
          "@id": "schema:PropertyValue"
        }
      ]
    },
    {
      "@id": "m4ml:hyperparameterValue",
      "@type": "rdf:Property",
      "rdfs:comment": "Hyperparameter values used to create this ML model. There should be a correspondence with the hyperparameters declared by the ML software used to create this ML model.",
      "rdfs:label": "hyperparameterValue",
      "schema:domainIncludes": [
        {
          "@id": "m4ml:MLModel"
        }
      ],
      "schema:rangeIncludes": [
         {
           "@id": "schema:PropertyValue"
         }
      ]
    },    
    {
      "@id": "m4ml:mlAlgorithm",
      "@type": "rdf:Property",
      "rdfs:comment": "ML algorithm used to solve the task. For instance logistic regression or random forests.",
      "rdfs:label": "mlAlgorithm",
      "schema:domainIncludes": [
        {
          "@id": "m4ml:MLSoftwareSourceCode"
        },
        {
          "@id": "m4ml:MLSoftwareApplication"
        },
        {
          "@id": "m4ml:MLModel"
        }
      ],
      "schema:rangeIncludes": [
        {
          "@id": "schema:Text"
        },
        {
          "@id": "schema:DefinedTerm"
        }
      ]
    },
    {
      "@id": "m4ml:mlTask",
      "@type": "rdf:Property",
      "rdfs:comment": "ML task addressed by this Ml software or model. For instance binary classification.",
      "rdfs:label": "mlTask",
      "schema:domainIncludes": [
        {
          "@id": "m4ml:MLSoftwareSourceCode"
        },
        {
          "@id": "m4ml:MLSoftwareApplication"
        },
        {
          "@id": "m4ml:MLModel"
        }
      ],
      "schema:rangeIncludes": [
        {
          "@id": "schema:Text"
        },
        {
          "@id": "schema:DefinedTerm"
        }
      ]
    },
    {
      "@id": "m4ml:optimizedFor",
      "@type": "rdf:Property",
      "rdfs:comment": "AI-ready dataset (after pre-processing) used by the ML software for the training and optimization of this ML model.",
      "rdfs:label": "optimizedFor",
      "schema:domainIncludes": [
        {
          "@id": "m4ml:MLModel"
        }
      ],
      "schema:rangeIncludes": [
         {
           "@id": "schema:Dataset"
         }
      ]
    },
    {
      "@id": "m4ml:retrainedBy",
      "@type": "rdf:Property",
      "rdfs:comment": "ML software used to re-train this ML model.",
      "rdfs:label": "retrainedBy",
      "schema:domainIncludes": [
        {
          "@id": "m4ml:MLModel"
        }
      ],
      "schema:rangeIncludes": [
         {
           "@id": "m4ml:MLSoftwareSourceCode"
         },
         {
          "@id": "m4ml:MLSoftwareApplication"
        }
      ]
    },
    {
      "@id": "m4ml:generatesOutput",
      "@type": "rdf:Property",
      "rdfs:comment": "ML model generated by this optimization action.",
      "rdfs:label": "generatesOutput",
      "schema:domainIncludes": [
        {
          "@id": "m4ml:MLModelOptimizationAction"
        }
      ],
      "schema:rangeIncludes": [
         {
           "@id": "m4ml:MLModel"
         },
         {
          "@id": "schema:CreativeWork"
        }
      ]
    },
    {
      "@id": "m4ml:validatesMLModel",
      "@type": "rdf:Property",
      "rdfs:comment": "ML model validated by this validation action.",
      "rdfs:label": "validatesMLModel",
      "schema:domainIncludes": [
        {
          "@id": "m4ml:MLModelValidationAction"
        }
      ],
      "schema:rangeIncludes": [
         {
           "@id": "m4ml:MLModel"
         }
      ]
    },
    {
      "@id": "m4ml:validationData",
      "@type": "rdf:Property",
      "rdfs:comment": "AI-ready dataset (after pre-processing) used by the ML validation action to perform an external validation with an unseen dataset.",
      "rdfs:label": "validationData",
      "schema:domainIncludes": [
        {
          "@id": "m4ml:MLModelValidationAction"
        }
      ],
      "schema:rangeIncludes": [
         {
           "@id": "schema:Dataset"
         }
      ]
    },


    {
      "@id": "bs:input",
      "@type": "rdf:Property",
      "rdfs:comment": "Specification of a consumed input.",
      "rdfs:label": "input",
      "schema:domainIncludes": [
        {
          "@id": "m4ml:MLSoftwareSourceCode"
        },
        {
          "@id": "m4ml:MLSoftwareApplication"
        }
      ],
      "schema:rangeIncludes": [
        {
          "@id": "bs:FormalParameter"
        }
      ]
    },
    {
      "@id": "bs:output",
      "@type": "rdf:Property",
      "rdfs:comment": "Specification of a produced output.",
      "rdfs:label": "output",
      "schema:domainIncludes": [
        {
          "@id": "m4ml:MLSoftwareSourceCode"
        },
        {
          "@id": "m4ml:MLSoftwareApplication"
        }
      ],
      "schema:rangeIncludes": [
        {
          "@id": "bs:FormalParameter"
        }
      ]
    },


    {
      "@id": "m4ml:ethicalLegalSocial",
      "@type": "rdf:Property",
      "rdfs:comment": "Considerations wrt ethical, legal and social aspects.",
      "rdfs:label": "ethicalLegalSocial",
      "schema:domainIncludes": [
        {
          "@id": "m4ml:MLSoftwareSourceCode"
        },
        {
          "@id": "m4ml:MLSoftwareApplication"
        },
        {
          "@id": "m4ml:MLModel"
        }
      ],
      "schema:rangeIncludes": [
        {
          "@id": "schema:Text"
        }
      ]
    },
    {
      "@id": "m4ml:intendedUse",
      "@type": "rdf:Property",
      "rdfs:comment": "Purpose and intended use stated to enable users to make a decision as to the suitability of this creative work (e.g., lab protocol, machine learning model, software) to their experimental problem or own use case.",
      "rdfs:label": "intendedUse",
      "schema:domainIncludes": [
        {
          "@id": "m4ml:MLSoftwareSourceCode"
        },
        {
          "@id": "m4ml:MLSoftwareApplication"
        },
        {
          "@id": "m4ml:MLModel"
        }
      ],
      "schema:rangeIncludes": [
        {
          "@id": "schema:Text"
        },
        {
          "@id": "schema:URL"
        },
        {
          "@id": "schema:DefinedTerm"
        }
      ]
    },


    {
      "@id": "codemeta:contIntegration",
      "@type": "rdf:Property",
      "rdfs:comment": "Link to continuous integration service.",
      "rdfs:label": "contIntegration",
      "schema:domainIncludes": [
        {
          "@id": "m4ml:MLSoftwareSourceCode"
        },
        {
          "@id": "m4ml:MLSoftwareApplication"
        },
        {
          "@id": "m4ml:MLModel"
        }
      ],
      "schema:rangeIncludes": [
        {
          "@id": "schema:URL"
        }
      ]
    },
    {
      "@id": "codemeta:buildInstructions",
      "@type": "rdf:Property",
      "rdfs:comment": "Link to installation instructions/documentation",
      "rdfs:label": "buildInstructions",
      "schema:domainIncludes": [
        {
          "@id": "m4ml:MLSoftwareSourceCode"
        },
        {
          "@id": "m4ml:MLSoftwareApplication"
        },
        {
          "@id": "m4ml:MLModel"
        }
      ],
      "schema:rangeIncludes": [
        {
          "@id": "schema:URL"
        }
      ]
    },
    {
      "@id": "codemeta:developmentStatus",
      "@type": "rdf:Property",
      "rdfs:comment": "Description of development status, e.g. Active, inactive, suspended. See <a href='http://www.repostatus.org/' target='_blank'>repostatus.org</a>",
      "rdfs:label": "developmentStatus",
      "schema:domainIncludes": [
        {
          "@id": "m4ml:MLSoftwareSourceCode"
        },
        {
          "@id": "m4ml:MLSoftwareApplication"
        },
        {
          "@id": "m4ml:MLModel"
        }
      ],
      "schema:rangeIncludes": [
        {
          "@id": "schema:Text"
        }
      ]
    },
    {
      "@id": "codemeta:embargoDate",
      "@type": "rdf:Property",
      "rdfs:comment": "Software may be embargoed from public access until a specified date (e.g. pending publication, 1 year from publication).",
      "rdfs:label": "embargoDate",
      "schema:domainIncludes": [
        {
          "@id": "m4ml:MLSoftwareSourceCode"
        },
        {
          "@id": "m4ml:MLSoftwareApplication"
        },
        {
          "@id": "m4ml:MLModel"
        }
      ],
      "schema:rangeIncludes": [
        {
          "@id": "schema:Date"
        }
      ]
    },
    {
      "@id": "codemeta:issueTracker",
      "@type": "rdf:Property",
      "rdfs:comment": "Link to software bug reporting or issue tracking system.",
      "rdfs:label": "issueTracker",
      "schema:domainIncludes": [
        {
          "@id": "m4ml:MLSoftwareSourceCode"
        },
        {
          "@id": "m4ml:MLSoftwareApplication"
        },
        {
          "@id": "m4ml:MLModel"
        }
      ],
      "schema:rangeIncludes": [
        {
          "@id": "schema:URL"
        }
      ]
    },
    {
      "@id": "codemeta:referencePublication",
      "@type": "rdf:Property",
      "rdfs:comment": "An academic publication related to the software.",
      "rdfs:label": "referencePublication",
      "schema:domainIncludes": [
        {
          "@id": "m4ml:MLSoftwareSourceCode"
        },
        {
          "@id": "m4ml:MLSoftwareApplication"
        },
        {
          "@id": "m4ml:MLModel"
        }
      ],
      "schema:rangeIncludes": [
        {
          "@id": "schema:ScholarlyArticle"
        }
      ]
    },
    {
      "@id": "codemeta:readme",
      "@type": "rdf:Property",
      "rdfs:comment": "Link to software Readme file",
      "rdfs:label": "readme",
      "schema:domainIncludes": [
        {
          "@id": "m4ml:MLSoftwareSourceCode"
        },
        {
          "@id": "m4ml:MLSoftwareApplication"
        },
        {
          "@id": "m4ml:MLModel"
        }
      ],
      "schema:rangeIncludes": [
        {
          "@id": "schema:URL"
        }
      ]
    }
  ]
}
